update pointers annotated with the C type

cogent/isa/UpdateSemantics.thy
@@ -14,44 +14,44 @@ theory UpdateSemantics
   imports Cogent
 begin
 
-datatype ('f, 'a, 'l) uval = UPrim lit
-                           | UProduct "('f,'a,'l) uval" "('f,'a,'l) uval"
-                           | USum name "('f,'a,'l) uval" "(name \<times> repr) list"
-                           | URecord "(('f,'a,'l) uval \<times> repr) list"
+datatype ('f, 'a, 'l, 't) uval = UPrim lit
+                           | UProduct "('f,'a,'l,'t) uval" "('f,'a,'l,'t) uval"
+                           | USum name "('f,'a,'l,'t) uval" "(name \<times> repr) list"
+                           | URecord "(('f,'a,'l,'t) uval \<times> repr) list"
                            | UAbstract "'a"
                            | UFunction "'f expr" "type list"
                            | UAFunction "'f" "type list"
                            | UUnit
-                           | UPtr "'l" repr
+                           | UPtr "'l" repr 't
 
 (* NB: The "type" in the store is just a tag used for the C proofs.
  *     The u_sem rules simply carry this tag along into the updated store. *)
-type_synonym ('f, 'a, 'l) store = "'l \<Rightarrow> ('f, 'a, 'l) uval option"
+type_synonym ('f, 'a, 'l, 't) store = "'l \<Rightarrow> ('f, 'a, 'l, 't) uval option"
 
 
-type_synonym ('f,'a,'l) ufundef = "('f,'a,'l) store \<times> ('f,'a,'l) uval
-                                 \<Rightarrow> ('f,'a,'l) store \<times> ('f,'a,'l) uval
+type_synonym ('f,'a,'l,'t) ufundef = "('f,'a,'l,'t) store \<times> ('f,'a,'l,'t) uval
+                                 \<Rightarrow> ('f,'a,'l,'t) store \<times> ('f,'a,'l,'t) uval
                                  \<Rightarrow> bool"
 
-type_synonym ('f, 'a, 'l) uabsfuns = "'f \<Rightarrow> ('f, 'a, 'l) ufundef"
+type_synonym ('f, 'a, 'l, 't) uabsfuns = "'f \<Rightarrow> ('f, 'a, 'l, 't) ufundef"
 
-definition eval_prim_u :: "prim_op \<Rightarrow> ('f, 'a, 'l) uval list \<Rightarrow> ('f, 'a, 'l) uval"
+definition eval_prim_u :: "prim_op \<Rightarrow> ('f, 'a, 'l, 't) uval list \<Rightarrow> ('f, 'a, 'l, 't) uval"
 where
   "eval_prim_u pop xs = UPrim (eval_prim_op pop (map (\<lambda>vv. case vv of UPrim v \<Rightarrow> v | _ \<Rightarrow> LBool False) xs))"
 
 
 
 
-inductive u_sem :: "('f,'a,'l) uabsfuns
-                  \<Rightarrow> ('f,'a,'l) uval env
-                  \<Rightarrow> ('f,'a,'l) store \<times> 'f expr
-                  \<Rightarrow> ('f,'a,'l) store \<times> ('f,'a,'l) uval
+inductive u_sem :: "('f,'a,'l,'t) uabsfuns
+                  \<Rightarrow> ('f,'a,'l,'t) uval env
+                  \<Rightarrow> ('f,'a,'l,'t) store \<times> 'f expr
+                  \<Rightarrow> ('f,'a,'l,'t) store \<times> ('f,'a,'l,'t) uval
                   \<Rightarrow> bool"
           ("_, _ \<turnstile> _ \<Down>! _" [30,0,0,20] 60)
-and       u_sem_all :: "('f,'a,'l) uabsfuns
-                      \<Rightarrow> ('f,'a,'l) uval env
-                      \<Rightarrow> ('f,'a,'l) store \<times> 'f expr list
-                      \<Rightarrow> ('f,'a,'l) store \<times> ('f,'a,'l) uval list
+and       u_sem_all :: "('f,'a,'l,'t) uabsfuns
+                      \<Rightarrow> ('f,'a,'l,'t) uval env
+                      \<Rightarrow> ('f,'a,'l,'t) store \<times> 'f expr list
+                      \<Rightarrow> ('f,'a,'l,'t) store \<times> ('f,'a,'l,'t) uval list
                       \<Rightarrow> bool"
           ("_, _ \<turnstile>* _ \<Down>! _" [30,0,0,20] 60)
 where
@@ -86,7 +86,7 @@ where
 | u_sem_member  : "\<lbrakk> \<xi> , \<gamma> \<turnstile> (\<sigma>, e) \<Down>! (\<sigma>', URecord fs)
                    \<rbrakk> \<Longrightarrow> \<xi> , \<gamma> \<turnstile> (\<sigma>, Member e f) \<Down>! (\<sigma>', fst (fs ! f))"
 
-| u_sem_memb_b  : "\<lbrakk> \<xi> , \<gamma> \<turnstile> (\<sigma>, e) \<Down>! (\<sigma>', UPtr p r)
+| u_sem_memb_b  : "\<lbrakk> \<xi> , \<gamma> \<turnstile> (\<sigma>, e) \<Down>! (\<sigma>', UPtr p r tyC)
                    ; \<sigma>' p = Some (URecord fs)
                    \<rbrakk> \<Longrightarrow> \<xi> , \<gamma> \<turnstile> (\<sigma>, Member e f) \<Down>! (\<sigma>', fst (fs ! f))"
 
@@ -123,20 +123,20 @@ where
 | u_sem_struct  : "\<lbrakk> \<xi> , \<gamma> \<turnstile>* (\<sigma>, xs) \<Down>! (\<sigma>', vs)
                    \<rbrakk> \<Longrightarrow> \<xi> , \<gamma> \<turnstile> (\<sigma>, Struct ts xs) \<Down>! (\<sigma>', URecord (zip vs (map type_repr ts)))"
 
-| u_sem_take    : "\<lbrakk> \<xi> , \<gamma> \<turnstile> (\<sigma>, x) \<Down>! (\<sigma>', UPtr p r)
+| u_sem_take    : "\<lbrakk> \<xi> , \<gamma> \<turnstile> (\<sigma>, x) \<Down>! (\<sigma>', UPtr p r tyC)
                    ; \<sigma>' p = Some (URecord fs)
-                   ; \<xi> , (fst (fs ! f) # UPtr p r # \<gamma>) \<turnstile> (\<sigma>', e) \<Down>! st
+                   ; \<xi> , (fst (fs ! f) # UPtr p r tyC # \<gamma>) \<turnstile> (\<sigma>', e) \<Down>! st
                    \<rbrakk> \<Longrightarrow> \<xi> , \<gamma> \<turnstile> (\<sigma>, Take x f e) \<Down>! st"
 
 | u_sem_take_ub : "\<lbrakk> \<xi> , \<gamma> \<turnstile> (\<sigma>, x) \<Down>! (\<sigma>', URecord fs)
                    ; \<xi> , (fst (fs ! f) # URecord fs # \<gamma>) \<turnstile> (\<sigma>', e) \<Down>! st
                    \<rbrakk> \<Longrightarrow> \<xi> , \<gamma> \<turnstile> (\<sigma>, Take x f e) \<Down>! st"
 
-| u_sem_put     : "\<lbrakk> \<xi> , \<gamma> \<turnstile> (\<sigma>, x) \<Down>! (\<sigma>', UPtr p r)
+| u_sem_put     : "\<lbrakk> \<xi> , \<gamma> \<turnstile> (\<sigma>, x) \<Down>! (\<sigma>', UPtr p r tyC)
                    ; \<sigma>' p = Some (URecord fs)
                    ; \<xi> , \<gamma> \<turnstile> (\<sigma>', e) \<Down>! (\<sigma>'', e')
                    \<rbrakk> \<Longrightarrow> \<xi> , \<gamma> \<turnstile> (\<sigma>, Put x f e)
-                      \<Down>! (\<sigma>'' (p := Some (URecord (fs [ f := (e', snd (fs ! f) )]))), UPtr p r)"
+                      \<Down>! (\<sigma>'' (p := Some (URecord (fs [ f := (e', snd (fs ! f) )]))), UPtr p r tyC)"
 
 | u_sem_put_ub  : "\<lbrakk> \<xi> , \<gamma> \<turnstile> (\<sigma>, x) \<Down>! (\<sigma>', URecord fs)
                    ; \<xi> , \<gamma> \<turnstile> (\<sigma>', e) \<Down>! (\<sigma>'', e')
@@ -173,7 +173,7 @@ locale update_sem =
 
 context update_sem begin
 
-fun uval_repr :: "('f, 'a, 'l) uval \<Rightarrow> repr" where
+fun uval_repr :: "('f, 'a, 'l, 't) uval \<Rightarrow> repr" where
   "uval_repr (UPrim lit) = RPrim (lit_type lit)"
 | "uval_repr (UProduct a b) = RProduct (uval_repr a) (uval_repr b)"
 | "uval_repr (USum a b reprs) = RSum reprs"
@@ -182,9 +182,9 @@ fun uval_repr :: "('f, 'a, 'l) uval \<Rightarrow> repr" where
 | "uval_repr (UFunction _ _) = RFun"
 | "uval_repr (UAFunction _ _) = RFun"
 | "uval_repr (UUnit) = RUnit"
-| "uval_repr (UPtr p r) = RPtr r"
+| "uval_repr (UPtr p r _) = RPtr r"
 
-fun uval_repr_deep :: "('f, 'a, 'l) uval \<Rightarrow> repr" where
+fun uval_repr_deep :: "('f, 'a, 'l, 't) uval \<Rightarrow> repr" where
   "uval_repr_deep (UPrim lit) = RPrim (lit_type lit)"
 | "uval_repr_deep (UProduct a b) = RProduct (uval_repr_deep a) (uval_repr_deep b)"
 | "uval_repr_deep (USum a b reprs) = RSum reprs"
@@ -193,18 +193,18 @@ fun uval_repr_deep :: "('f, 'a, 'l) uval \<Rightarrow> repr" where
 | "uval_repr_deep (UFunction _ _) = RFun"
 | "uval_repr_deep (UAFunction _ _) = RFun"
 | "uval_repr_deep (UUnit) = RUnit"
-| "uval_repr_deep (UPtr p r) = RPtr r"
+| "uval_repr_deep (UPtr p r _) = RPtr r"
 
 inductive uval_typing :: "('f \<Rightarrow> poly_type)
-                       \<Rightarrow> ('f, 'a, 'l) store
-                       \<Rightarrow> ('f, 'a, 'l) uval
+                       \<Rightarrow> ('f, 'a, 'l, 't) store
+                       \<Rightarrow> ('f, 'a, 'l, 't) uval
                        \<Rightarrow> type
                        \<Rightarrow> 'l set
                        \<Rightarrow> 'l set
                        \<Rightarrow> bool"  ("_, _ \<turnstile> _ :u _ \<langle>_, _\<rangle>" [30,0,0,0,20] 80)
 and uval_typing_record :: "('f \<Rightarrow> poly_type)
-                        \<Rightarrow> ('f, 'a, 'l) store
-                        \<Rightarrow> (('f, 'a, 'l) uval \<times> repr) list
+                        \<Rightarrow> ('f, 'a, 'l, 't) store
+                        \<Rightarrow> (('f, 'a, 'l, 't) uval \<times> repr) list
                         \<Rightarrow> (name \<times> type \<times> record_state) list
                         \<Rightarrow> 'l set
                         \<Rightarrow> 'l set
@@ -252,26 +252,26 @@ and uval_typing_record :: "('f \<Rightarrow> poly_type)
 | u_t_p_rec_ro : "\<lbrakk> \<Xi>, \<sigma> \<turnstile>* fs :ur ts \<langle>r, {}\<rangle>
                   ; \<sigma> l = Some (URecord fs)
                   ; distinct (map fst ts)
-                  \<rbrakk> \<Longrightarrow> \<Xi>, \<sigma> \<turnstile> UPtr l (RRecord (map (type_repr \<circ> fst \<circ> snd) ts)) :u TRecord ts (Boxed ReadOnly ptrl) \<langle>insert l r, {}\<rangle>"
+                  \<rbrakk> \<Longrightarrow> \<Xi>, \<sigma> \<turnstile> UPtr l (RRecord (map (type_repr \<circ> fst \<circ> snd) ts)) tyC :u TRecord ts (Boxed ReadOnly ptrl) \<langle>insert l r, {}\<rangle>"
 
 | u_t_p_rec_w  : "\<lbrakk> \<Xi>, \<sigma> \<turnstile>* fs :ur ts \<langle>r, w\<rangle>
                   ; \<sigma> l = Some (URecord fs)
                   ; l \<notin> (w \<union> r)
                   ; distinct (map fst ts)
-                  \<rbrakk> \<Longrightarrow> \<Xi>, \<sigma> \<turnstile> UPtr l (RRecord (map (type_repr \<circ> fst \<circ> snd) ts)) :u TRecord ts (Boxed Writable ptrl) \<langle>r, insert l w\<rangle>"
+                  \<rbrakk> \<Longrightarrow> \<Xi>, \<sigma> \<turnstile> UPtr l (RRecord (map (type_repr \<circ> fst \<circ> snd) ts)) tyC :u TRecord ts (Boxed Writable ptrl) \<langle>r, insert l w\<rangle>"
 
 | u_t_p_abs_ro : "\<lbrakk> s = Boxed ReadOnly ptrl
                   ; abs_typing a n ts s r {}
                   ; [] \<turnstile>* ts wellformed
                   ; \<sigma> l = Some (UAbstract a)
-                  \<rbrakk> \<Longrightarrow> \<Xi>, \<sigma> \<turnstile> UPtr l (RCon n (map type_repr ts)) :u TCon n ts s \<langle>insert l r, {}\<rangle>"
+                  \<rbrakk> \<Longrightarrow> \<Xi>, \<sigma> \<turnstile> UPtr l (RCon n (map type_repr ts)) tyC :u TCon n ts s \<langle>insert l r, {}\<rangle>"
 
 | u_t_p_abs_w  : "\<lbrakk> s = Boxed Writable ptrl
                   ; abs_typing a n ts s r w
                   ; [] \<turnstile>* ts wellformed
                   ; \<sigma> l = Some (UAbstract a)
                   ; l \<notin> (w \<union> r)
-                  \<rbrakk> \<Longrightarrow> \<Xi>, \<sigma> \<turnstile> UPtr l (RCon n (map type_repr ts)) :u TCon n ts s \<langle>r, insert l w\<rangle>"
+                  \<rbrakk> \<Longrightarrow> \<Xi>, \<sigma> \<turnstile> UPtr l (RCon n (map type_repr ts)) tyC :u TCon n ts s \<langle>r, insert l w\<rangle>"
 
 | u_t_r_empty  : "\<Xi>, \<sigma> \<turnstile>* [] :ur [] \<langle>{}, {}\<rangle>"
 | u_t_r_cons1  : "\<lbrakk> \<Xi>, \<sigma> \<turnstile>  x  :u  t  \<langle>r , w \<rangle>
@@ -298,13 +298,13 @@ inductive_cases u_t_afunE     [elim] : "\<Xi>, \<sigma> \<turnstile> UAFunction 
 inductive_cases u_t_sumE      [elim] : "\<Xi>, \<sigma> \<turnstile> v :u TSum \<tau>s \<langle>r, w\<rangle>"
 inductive_cases u_t_productE  [elim] : "\<Xi>, \<sigma> \<turnstile> UProduct a b :u TProduct \<tau> \<rho> \<langle>r, w\<rangle>"
 inductive_cases u_t_recE      [elim] : "\<Xi>, \<sigma> \<turnstile> URecord fs :u \<tau> \<langle>r, w\<rangle>"
-inductive_cases u_t_p_recE    [elim] : "\<Xi>, \<sigma> \<turnstile> UPtr p rp :u TRecord fs s \<langle>r, w\<rangle>"
+inductive_cases u_t_p_recE    [elim] : "\<Xi>, \<sigma> \<turnstile> UPtr p rp tyC :u TRecord fs s \<langle>r, w\<rangle>"
 inductive_cases u_t_r_emptyE  [elim] : "\<Xi>, \<sigma> \<turnstile>* [] :ur \<tau>s \<langle>r, w\<rangle>"
 inductive_cases u_t_r_consE   [elim] : "\<Xi>, \<sigma> \<turnstile>* (x # xs) :ur \<tau>s \<langle>r, w\<rangle>"
 
 inductive uval_typing_all :: "('f \<Rightarrow> poly_type)
-                            \<Rightarrow> ('f, 'a, 'l) store
-                            \<Rightarrow> ('f, 'a, 'l) uval list
+                            \<Rightarrow> ('f, 'a, 'l, 't) store
+                            \<Rightarrow> ('f, 'a, 'l, 't) uval list
                             \<Rightarrow> type list
                             \<Rightarrow> 'l set
                             \<Rightarrow> 'l set
@@ -319,8 +319,8 @@ inductive uval_typing_all :: "('f \<Rightarrow> poly_type)
                     \<rbrakk> \<Longrightarrow> \<Xi>, \<sigma> \<turnstile>* (x # xs) :u (t # ts) \<langle>r \<union> r', w \<union> w'\<rangle>"
 
 inductive matches_ptrs :: "('f \<Rightarrow> poly_type)
-                         \<Rightarrow> ('f, 'a, 'l) store
-                         \<Rightarrow> ('f, 'a, 'l) uval env
+                         \<Rightarrow> ('f, 'a, 'l, 't) store
+                         \<Rightarrow> ('f, 'a, 'l, 't) uval env
                          \<Rightarrow> ctx
                          \<Rightarrow> 'l set
                          \<Rightarrow> 'l set
@@ -341,13 +341,13 @@ inductive matches_ptrs :: "('f \<Rightarrow> poly_type)
 inductive_cases matches_ptrs_consE: "\<Xi>, \<sigma> \<turnstile> \<gamma> matches (\<tau> # \<tau>s) \<langle> r , w \<rangle>"
 
 
-definition frame :: "('f, 'a, 'l) store \<Rightarrow> 'l set \<Rightarrow> ('f, 'a, 'l) store \<Rightarrow> 'l set \<Rightarrow> bool"
+definition frame :: "('f, 'a, 'l, 't) store \<Rightarrow> 'l set \<Rightarrow> ('f, 'a, 'l, 't) store \<Rightarrow> 'l set \<Rightarrow> bool"
            where
   "frame \<sigma> pi \<sigma>' po \<equiv> \<forall>p. (p \<in> pi \<and> p \<notin> po \<longrightarrow> \<sigma>' p = None)
                        \<and>  (p \<notin> pi \<and> p \<in> po \<longrightarrow> \<sigma>  p = None)
                        \<and>  (p \<notin> pi \<and> p \<notin> po \<longrightarrow> \<sigma>  p = \<sigma>' p)"
 
-definition proc_env_matches_ptrs :: "(('f,'a,'l) uabsfuns) \<Rightarrow> ('f \<Rightarrow> poly_type) \<Rightarrow> bool"
+definition proc_env_matches_ptrs :: "(('f,'a,'l,'t) uabsfuns) \<Rightarrow> ('f \<Rightarrow> poly_type) \<Rightarrow> bool"
            ("_ matches-u _" [30,20] 60) where
   "\<xi> matches-u \<Xi> \<equiv> (\<forall> f. let (K, \<tau>i, \<tau>o) = \<Xi> f
                           in (\<forall> \<sigma> \<sigma>' \<tau>s v v' r w. list_all2 (kinding []) \<tau>s K
@@ -555,27 +555,27 @@ next
   case u_t_abstract then show ?case
     by (force intro: uval_typing_uval_typing_record.intros bang_wellformed abs_typing_bang[where s = Unboxed, simplified])
 next
-  case (u_t_p_rec_ro \<Xi> \<sigma> fs ts r l ptrl)
-  moreover have "\<Xi>, \<sigma> \<turnstile> UPtr l (RRecord (map (type_repr \<circ> fst \<circ> snd \<circ> apsnd (apfst bang)) ts)) :u TRecord (map (apsnd (apfst bang)) ts) (Boxed ReadOnly ptrl) \<langle>insert l r, {}\<rangle>"
+  case (u_t_p_rec_ro \<Xi> \<sigma> fs ts r l tyC ptrl)
+  moreover have "\<Xi>, \<sigma> \<turnstile> UPtr l (RRecord (map (type_repr \<circ> fst \<circ> snd \<circ> apsnd (apfst bang)) ts)) tyC :u TRecord (map (apsnd (apfst bang)) ts) (Boxed ReadOnly ptrl) \<langle>insert l r, {}\<rangle>"
     using u_t_p_rec_ro
     by (fastforce dest: uval_typing_to_wellformed(2) uval_typing_uval_typing_record.u_t_p_rec_ro)
   ultimately show ?case
     by (force dest: uval_typing_to_wellformed(2) simp add: fst_apfst_compcomp snd_apsnd_compcomp map_snd3_keep)
 next
-  case (u_t_p_rec_w \<Xi> \<sigma> fs ts r w l ptrl)
-  moreover have "\<Xi>, \<sigma> \<turnstile> UPtr l (RRecord (map (type_repr \<circ> fst \<circ> snd \<circ> apsnd (apfst bang)) ts)) :u TRecord (map (apsnd (apfst bang)) ts) (Boxed ReadOnly ptrl) \<langle>insert l (r \<union> w), {}\<rangle>"
+  case (u_t_p_rec_w \<Xi> \<sigma> fs ts r w l tyC ptrl)
+  moreover have "\<Xi>, \<sigma> \<turnstile> UPtr l (RRecord (map (type_repr \<circ> fst \<circ> snd \<circ> apsnd (apfst bang)) ts)) tyC :u TRecord (map (apsnd (apfst bang)) ts) (Boxed ReadOnly ptrl) \<langle>insert l (r \<union> w), {}\<rangle>"
     using u_t_p_rec_w uval_typing_uval_typing_record.u_t_p_rec_ro by fastforce
   ultimately show ?case
     by (auto dest!: uval_typing_to_wellformed(2) simp add: fst_apfst_compcomp snd_apsnd_compcomp map_snd3_keep)
 next
-  case (u_t_p_abs_ro s ptrl a n ts r \<sigma> l \<Xi>)
-  then have "\<Xi>, \<sigma> \<turnstile> UPtr l (RCon n (map type_repr (map bang ts))) :u TCon n (map bang ts) (Boxed ReadOnly ptrl) \<langle>insert l r, {}\<rangle>"
+  case (u_t_p_abs_ro s ptrl a n ts r \<sigma> l \<Xi> tyC)
+  then have "\<Xi>, \<sigma> \<turnstile> UPtr l (RCon n (map type_repr (map bang ts))) tyC :u TCon n (map bang ts) (Boxed ReadOnly ptrl) \<langle>insert l r, {}\<rangle>"
     by (fastforce intro!: uval_typing_uval_typing_record.intros dest: abs_typing_bang bang_kind(2) bang_wellformed)
   then show ?case
     using u_t_p_abs_ro by clarsimp
 next
-  case (u_t_p_abs_w s ptrl a n ts r w \<sigma> l \<Xi>)
-  then have "\<Xi>, \<sigma> \<turnstile> UPtr l (RCon n (map type_repr (map bang ts))) :u TCon n (map bang ts) (Boxed ReadOnly ptrl) \<langle>insert l (r \<union> w), {}\<rangle>"
+  case (u_t_p_abs_w s ptrl a n ts r w \<sigma> l \<Xi> tyC)
+  then have "\<Xi>, \<sigma> \<turnstile> UPtr l (RCon n (map type_repr (map bang ts))) tyC :u TCon n (map bang ts) (Boxed ReadOnly ptrl) \<langle>insert l (r \<union> w), {}\<rangle>"
     by (fastforce intro!: uval_typing_uval_typing_record.intros dest: abs_typing_bang bang_kind(2) bang_wellformed)
   then show ?case
     using u_t_p_abs_w by clarsimp
@@ -1603,7 +1603,7 @@ next
     using u_t_function.prems apply (cases rule: subtyping.cases)
     using u_t_function by (fastforce simp add: subtyping_trans uval_typing_uval_typing_record.intros)
 next
-  case (u_t_p_rec_ro \<Xi> \<sigma> fs ts r l ptrl)
+  case (u_t_p_rec_ro \<Xi> \<sigma> fs ts r l tyC ptrl)
   obtain ts' where elims:
     "t' = TRecord ts' (Boxed ReadOnly ptrl)"
     "map fst ts = map fst ts'"
@@ -1624,7 +1624,7 @@ next
     using u_t_p_rec_ro elims fields repr_same uval_typing_uval_typing_record.u_t_p_rec_ro
     by (metis (no_types, lifting) insert_mono)
 next
-  case (u_t_p_rec_w \<Xi> \<sigma> fs ts r w l ptrl)
+  case (u_t_p_rec_w \<Xi> \<sigma> fs ts r w l tyC ptrl)
   obtain ts' where elims:
     "t' = TRecord ts' (Boxed Writable ptrl)"
     "map fst ts = map fst ts'"
@@ -1779,7 +1779,7 @@ lemma u_t_p_rec_w':
     and "l \<notin> w \<union> r"
     and "rp = (RRecord (map (type_repr \<circ> fst \<circ> snd) ts)) "
     and "distinct (map fst ts)"
-  shows "\<Xi>, \<sigma> \<turnstile> UPtr l rp :u TRecord ts (Boxed Writable ptrl) \<langle> r, insert l w \<rangle>"
+  shows "\<Xi>, \<sigma> \<turnstile> UPtr l rp tyC :u TRecord ts (Boxed Writable ptrl) \<langle> r, insert l w \<rangle>"
   using assms
   by (auto intro: u_t_p_rec_w)
 
@@ -2332,7 +2332,7 @@ next case u_sem_memb_b
          , fastforce )
  done
 next
-  case (u_sem_take \<xi> \<gamma> \<sigma> x_spec \<sigma>'' pa ra fs f ea_spec)
+  case (u_sem_take \<xi> \<gamma> \<sigma> x_spec \<sigma>'' pa ra tyCa fs f ea_spec)
   then show ?case
   proof (cases e)
     case (Take x f' ea)
@@ -2369,7 +2369,7 @@ next
 
     obtain r1' w1pa'
       where IH1_lemmas:
-        "\<Xi>, \<sigma>'' \<turnstile> UPtr pa ra :u instantiate \<tau>s (TRecord ts s) \<langle>r1', w1pa'\<rangle>"
+        "\<Xi>, \<sigma>'' \<turnstile> UPtr pa ra tyCa :u instantiate \<tau>s (TRecord ts s) \<langle>r1', w1pa'\<rangle>"
         "r1' \<subseteq> r1"
         "frame \<sigma> w1 \<sigma>'' w1pa'"
       using u_sem_take.hyps(2) u_sem_take.prems ptrs_split_lemmas typing_e_elim_lemmas case_simps
@@ -2429,7 +2429,7 @@ next
     proof (cases taken)
       case Taken
 
-      have "\<Xi>, \<sigma>'' \<turnstile> fst (fs ! f') # UPtr pa ra # \<gamma>
+      have "\<Xi>, \<sigma>'' \<turnstile> fst (fs ! f') # UPtr pa ra tyCa # \<gamma>
             matches Some (instantiate \<tau>s t)
               # Some (TRecord ((map (\<lambda>(n, t, y). (n, instantiate \<tau>s t, y)) ts)[f' := (n, instantiate \<tau>s t, Taken)]) (Boxed Writable ptrl))
               # instantiate_ctx \<tau>s \<Gamma>2
@@ -2483,7 +2483,7 @@ next
       then have w1'''_is: "w1''' = w1'"
         by (simp add: utype_record_take_lemmas(4))
 
-      have "\<Xi>, \<sigma>'' \<turnstile> fst (fs ! f') # UPtr pa ra # \<gamma>
+      have "\<Xi>, \<sigma>'' \<turnstile> fst (fs ! f') # UPtr pa ra tyCa # \<gamma>
             matches Some (instantiate \<tau>s t)
               # Some (TRecord (map (\<lambda>(n, t, y). (n, instantiate \<tau>s t, y)) ts) (Boxed Writable ptrl))
               # instantiate_ctx \<tau>s \<Gamma>2
@@ -2777,7 +2777,7 @@ inductive_cases u_t_productE': "\<Xi>, \<sigma> \<turnstile> UProduct a b :u t \
 inductive_cases u_t_sumE': "\<Xi>, \<sigma> \<turnstile> USum c p ts :u t \<langle>r,w\<rangle>"
 inductive_cases u_t_absE: "\<Xi>, \<sigma> \<turnstile> UAbstract v :u t \<langle>r,w\<rangle>"
 inductive_cases u_t_funE': "\<Xi>, \<sigma> \<turnstile> UFunction f ts :u t \<langle>r,w\<rangle>"
-inductive_cases u_t_ptrE: "\<Xi>, \<sigma> \<turnstile> UPtr p rp :u t \<langle>r,w\<rangle>"
+inductive_cases u_t_ptrE: "\<Xi>, \<sigma> \<turnstile> UPtr p rp tyC :u t \<langle>r,w\<rangle>"
 
 lemma type_repr_heap:
 shows "\<lbrakk> \<Xi>, \<sigma> \<turnstile>  v  :u  t  \<langle>r, w\<rangle>; \<Xi>, \<sigma> \<turnstile>  v  :u  t'  \<langle>r', w'\<rangle> \<rbrakk> \<Longrightarrow> type_repr t = type_repr t'"
